Prove the ctx_inst obligation of on_constructor

pcuic/theories/PCUICArities.v
@@ -271,6 +271,32 @@ Proof.
     now rewrite sort_of_product_twice.
 Qed.
 
+Fixpoint sort_of_products us s :=
+  match us with
+  | [] => s
+  | u :: us => sort_of_products us (Universe.sort_of_product u s)
+  end.
+
+Lemma type_it_mkProd_or_LetIn_sorts {cf:checker_flags} Σ Γ Γ' us t s : 
+  wf Σ.1 ->
+  sorts_local_ctx (lift_typing typing) Σ Γ Γ' us ->
+  Σ ;;; Γ ,,, Γ' |- t : tSort s ->
+  Σ ;;; Γ |- it_mkProd_or_LetIn Γ' t : tSort (sort_of_products us s).
+Proof.
+  revert Γ us s t.
+  induction Γ'; simpl; auto; move=> Γ us s t wfΣ equ Ht.
+  - destruct us => //.
+  - destruct a as [na [b|] ty]; intuition auto.
+    * destruct a0 as [s' Hs].
+      eapply IHΓ'; eauto.
+      eapply (type_mkProd_or_LetIn _ _ {| decl_body := Some b |}); auto.
+      simpl. exact Hs.
+    * destruct us => //. destruct equ.
+      simpl.   
+      eapply IHΓ'; eauto.
+      apply (type_mkProd_or_LetIn _ _ {| decl_body := None |}) => /=; eauto.
+Qed.
+
 Lemma isType_wf_local {cf:checker_flags} {Σ Γ T} : isType Σ Γ T -> wf_local Σ Γ.
 Proof.
   move=> [s Hs].
